lean: tweak lean proof to kill one axiom.
The axiom about wf safety is unnecessary. It should (in principle) be
implied by the WF termination axiom, but this wasn't true because the
safety definition required there to be a valid instruction to execute
next even for final states. Weaken the safety to include final states as
well, then rewrite the axiom as a lemma and tweak the star_src_correct
proof to kill the final state case before proceeding with the usual
per-instruction correctness.

lean/src/jit.lean
@@ -7,11 +7,9 @@ This file contains the metatheory of JIT correctness.
 The main theorems are forward_simulation and backward_simulation, proved based
 on the following two sets of axioms.
 
-Three axioms are assumed to be correct (e.g., ensured by the Linux kernel):
+Two axioms are assumed to be correct (e.g., ensured by the Linux kernel):
 
 * wf_terminates: a program that passes the checker terminates.
-
-* wf_safe: a program that passes the checker is safe.
 
 * emit_correct: the output of the JIT contains the output of individual parts.
 
@@ -209,11 +207,12 @@ namespace source
   -- Initial state of a source program.
   constant init_state : INPUT → STATE
 
-  -- A safe state can always fetch an instruction from any reachable state.
+  -- A safe state can always fetch an instruction from any reachable state,
+  -- or it's the final state
   def safe (oracle : NONDET) (code : CODE) (s1 : STATE) : Prop :=
     ∀ s2 tr,
       star oracle code s1 s2 tr →
-      ∃ insn, code (pc_of s2) = some insn
+      (∃ insn, code (pc_of s2) = some insn) ∨ (∃ res, result_of s2 = some res)
 
   -- This captures the guarantees of the checker: a well-formed program passes
   -- the checker.
@@ -229,25 +228,35 @@ namespace source
         star oracle code (init_state i) s' tr ∧
         result_of s' = some res
 
-  -- A well-formed program is safe from the initial state.
-  --
-  -- This is assumed to hold.
-  axiom wf_safe :
-    ∀ (code : CODE) (i : INPUT),
-      wf code →
-      ∀ (oracle : NONDET),
-        safe oracle code (init_state i)
+  lemma final_safe :
+    ∀ oracle code s1 res,
+      result_of s1 = some res →
+      safe oracle code s1 :=
+  begin
+    dsimp [safe], intros, right,
+    induction a_1,
+    existsi res, assumption,
+    apply a_1_ih,
+    dsimp [machine.step] at *,
+    rw a at *,
+    cases a_1_a_1,
+    assumption,
+  end
 
-  -- A safe state can always take a step.
+  -- A safe state can always take a step if it's not final.
   lemma safe_self :
     ∀ (oracle : NONDET) (code : CODE) (s : STATE),
       safe oracle code s →
+      result_of s = none →
       ∃ (insn : INSN),
         code (pc_of s) = some insn :=
   begin
-    intros _ _ _ H1,
-    unfold safe at *,
-    apply H1, constructor,
+    intros,
+    dsimp [safe] at *,
+    specialize a s [] (by constructor),
+    cases a, assumption,
+    cases a, rw a_h at *,
+    contradiction,
   end
 
   -- A safe state is still safe after one step.
@@ -263,6 +272,72 @@ namespace source
     specialize H1 _ (tr ++ tr_1),
     apply H1,
     constructor; assumption,
+  end
+
+  lemma safe_star :
+    ∀ (oracle : NONDET) (code : CODE) (s₁ s₂ : STATE) (tr : TRACE),
+      safe oracle code s₁ →
+      star oracle code s₁ s₂ tr →
+      safe oracle code s₂ :=
+  begin
+    intros,
+    induction a_1, by assumption,
+    apply a_1_ih,
+    apply safe_step; assumption,
+  end
+
+  lemma safe_step_backwards :
+    ∀ (oracle : NONDET) (code : CODE) (s₁ s₂ : STATE) (tr : TRACE),
+      safe oracle code s₂ →
+      step oracle code s₁ = some (s₂, tr) →
+      safe oracle code s₁ :=
+  begin
+    intros,
+    dsimp [safe], intros,
+    revert s₂,
+    induction a_2; intros,
+    dsimp [step, machine.step] at *,
+    cases h4 : (result_of a_2); rw h4 at *; dsimp [machine.step._match_1] at *,
+    cases h5 : (code (pc_of a_2)); rw h5 at *,
+    contradiction,
+    left,
+    existsi val, reflexivity,
+    cases a_1,
+    right, existsi val, reflexivity,
+    dsimp [step] at a_1,
+    rw a_1 at *,
+    cases a_2_a_1,
+    let x := safe_star oracle code _ _ _ a a_2_a_2,
+    dsimp [safe] at x,
+    apply x,
+    apply machine.star.refl,
+  end
+
+  lemma terminates_safe :
+    ∀ oracle code s1 s2 tr res,
+      star oracle code s1 s2 tr →
+      result_of s2 = some res →
+      safe oracle code s1 :=
+  begin
+    intros,
+    induction a,
+    apply final_safe; assumption,
+    apply safe_step_backwards; try{assumption},
+    apply a_ih, assumption,
+  end
+
+  lemma wf_safe :
+    ∀ (code : CODE) (i : INPUT),
+      wf code →
+      ∀ (oracle : NONDET),
+        safe oracle code (init_state i) :=
+  begin
+    intros,
+    cases (wf_terminates oracle i code (by assumption)),
+    cases h,
+    cases h_h,
+    cases h_h_h,
+    apply terminates_safe; try{assumption},
   end
 
 end source
@@ -384,6 +459,15 @@ begin
   { intros _ _ _ related emitted,
     existsi σ_T, split, constructor, assumption, },
   intros _ _ _ related emitted,
+
+  cases hresult : (source.result_of s1),
+  tactic.swap,
+  { dsimp [machine.step] at *,
+    rw hresult at *,
+    cases step_S,
+    cases step_S,
+    apply IH; assumption,
+  },
 
   have hinsn : ∃ insn, code_S (source.pc_of s1) = some insn,
   {
